fix #288 fix isabelle realization for sets and fsets
This patch should solve the problem of realizations of sets and fsets.

lib/isabelle/Why3_Set.thy
@@ -10,6 +10,9 @@ section {* Potentially infinite sets *}
 definition complement :: "('a \<Rightarrow> bool) \<Rightarrow> 'a \<Rightarrow> bool" where
   "complement S v = Not (S v)"
 
+definition mapi :: "('a \<Rightarrow> 'b) \<Rightarrow> ('a \<Rightarrow> bool) \<Rightarrow> ('b \<Rightarrow> bool)" where
+  "mapi f s x = Set.member x (image f (Collect s))"
+
 why3_open "set/Set.xml"
   constants
     empty = bot
@@ -19,41 +22,30 @@ why3_open "set/Set.xml"
     inter = inf
     diff = minus
     complement = complement
-    choose = Eps
+    pick = Eps
     all = top
+    map = mapi
 
-why3_vc add_spec by (auto simp add: mem_def)
+why3_vc diff_def by (simp add: mem_def)
 
-why3_vc diff_def by simp
-
-why3_vc diff_spec by (simp add: mem_def)
-
-why3_vc inter_def by simp
+why3_vc inter_def by (simp add: mem_def)
 
 why3_vc is_empty_empty by (simp add: const_def mem_def set.Set.is_empty_def)
 
-why3_vc union_def by simp
+why3_vc union_def by (simp add: mem_def)
 
 why3_vc add_remove
   using assms
   by (simp add: fun_upd_idem_iff mem_def)
 
-why3_vc inter_spec by (simp add: mem_def)
-
 why3_vc remove_add by auto
 
-why3_vc union_spec
-  by (simp add: mem_def)
-
-why3_vc choose_spec
+why3_vc pick_def
   using assms
   by (auto simp add: mem_def is_empty_def intro: someI_ex)
 
-why3_vc remove_spec
-  by (simp add: mem_def)
-
 why3_vc subset_diff
-  by (simp add: diff_spec subset_def)
+  by (simp add: mem_def diff_def subset_def)
 
 why3_vc subset_refl
   by (simp add: subset_def)
@@ -63,14 +55,48 @@ why3_vc subset_trans
   by (simp add: subset_def)
 
 why3_vc subset_remove
-  by (simp add: remove_spec subset_def)
+  by (simp add: mem_def remove_def subset_def)
 
 why3_vc complement_def
-  by (simp add: complement_def)
+  by (simp add: mem_def complement_def)
 
 why3_vc extensionality
   using assms
   by (auto simp add: infix_eqeq_def mem_def)
+
+why3_vc map_def by (simp add: mem_def mapi_def image_iff)
+
+why3_vc mem_map
+  using assms
+  by (meson facts.map_def mem_def)
+
+why3_vc mem_singleton
+  by (metis assms const_def fun_upd_other mem_def) 
+
+why3_vc empty_is_empty
+  using assms
+  by (meson extensionality infix_eqeq_def is_empty_empty set.Set.is_empty_def)
+
+why3_vc subset_inter_1
+  by (simp add: set.Set.subset_def mem_def)
+
+why3_vc subset_inter_2
+  by (simp add: set.Set.subset_def mem_def)
+
+why3_vc subset_union_1
+  by (simp add: set.Set.subset_def mem_def)
+
+why3_vc subset_union_2
+  by (simp add: set.Set.subset_def mem_def)
+
+why3_vc disjoint_diff_eq
+  by (smt diff_def disjoint_def extensionality infix_eqeq_def mem_def)
+
+why3_vc disjoint_diff_s2
+  by (simp add: disjoint_def mem_def)
+
+why3_vc disjoint_inter_empty
+  by (simp add: disjoint_def mem_def set.Set.is_empty_def)
 
 why3_end
 
@@ -86,6 +112,9 @@ definition fchoose :: "'a fset \<Rightarrow> 'a" where
 definition is_empty :: "'a fset \<Rightarrow> bool" where
   "is_empty S = (S = fempty)"
 
+definition filter :: "'a fset \<Rightarrow> ('a \<Rightarrow> bool) \<Rightarrow> 'a fset" where
+  "filter S p = ffilter p S"
+
 why3_open "set/Fset.xml"
   constants
     mem = fmember
@@ -97,13 +126,13 @@ why3_open "set/Fset.xml"
     diff = minus
     choose = fchoose
     all = top
-    infix_eqeq = HOL.eq
-    subset = fsubset_eq
-    is_empty = is_empty
+    pick = fchoose
+    filter = filter
+    map = fimage
   types
-    set = fset
+    fset = fset
 
-why3_vc add_spec by simp
+why3_vc add_def by auto
 
 why3_vc add_remove
   using assms
@@ -111,35 +140,39 @@ why3_vc add_remove
 
 why3_vc remove_add by (simp add: fremove_def)
 
-why3_vc empty_def by (simp add: is_empty_def)
+why3_vc map_def by auto
 
-why3_vc inter_spec by simp
+why3_vc mem_map by (simp add: assms)
 
-why3_vc union_spec by simp
+why3_vc inter_def by simp
 
-why3_vc remove_spec by (auto simp add: fremove_def)
+why3_vc union_def by simp
 
-why3_vc subset_diff by auto
+why3_vc remove_def by (auto simp add: fremove_def)
 
-why3_vc subset_refl by simp
+why3_vc diff_def by auto
 
-why3_vc subset_trans
+why3_vc pick_def
   using assms
-  by simp
+  by (auto simp add: fchoose_def is_empty_def intro: someI_ex)
 
-why3_vc subset_remove by (auto simp add: fremove_def)
+why3_vc subset_diff by (simp add: Fset.subset_def)
+
+why3_vc subset_refl by (simp add: Fset.subset_def)
+
+why3_vc subset_trans 
+  using assms
+  by (simp add: Fset.subset_def)
+
+why3_vc subset_remove by (auto simp add: Fset.subset_def fremove_def)
 
 why3_vc subset_eq
-  using assms fcard_seteq by fastforce
-
-why3_vc subset_spec by auto
-
-why3_vc infix_eqeq_spec
-  by (simp add: fset_eq_iff)
+  using assms fcard_seteq
+  by (metis Fset.subset_def eq_imp_le fsubsetI of_nat_eq_iff)
 
 why3_vc extensionality
   using assms
-  by simp
+  by (simp add:  Fset.infix_eqeq_def fset_eqI)
 
 why3_vc cardinal1
 proof (cases s rule: fset_strong_cases)
@@ -161,36 +194,76 @@ next
   qed
 qed
 
-why3_vc cardinal_add
-  using assms
-  by (simp add: fcard_finsert_disjoint)
+why3_vc cardinal_add by (auto simp add: fcard_finsert_if finsert_absorb)
 
 why3_vc cardinal_empty by (simp add: is_empty_def)
 
 why3_vc cardinal_nonneg by simp
 
-why3_vc cardinal_remove
-proof -
-  from assms
-  have "1 \<le> fcard s"
-    by (cases s rule: fset_strong_cases)
-      (auto simp add: fcard_finsert_disjoint)
-  with assms show ?thesis
-    by (simp add: fremove_def)
-qed
+lemma cardinal_remove_in: 
+  "x |\<in>| s \<longrightarrow> int (fcard (fremove x s)) = int (fcard s) - 1"
+  by (smt cardinal_add(2) fminus_finsert_absorb fremove_def set_finsert)
+
+lemma cardinal_remove_out:
+  "x |\<notin>| s \<longrightarrow> int (fcard (fremove x s)) = int (fcard s)"
+  by (simp add: fremove_def)
+
+why3_vc cardinal_remove by (auto simp add: cardinal_remove_out cardinal_remove_in)
 
 why3_vc cardinal_subset
   using assms
-  by (simp add: fcard_mono)
+  by (simp add: Fset.subset_def fcard_mono fsubsetI)
 
-why3_vc diff_spec by simp
+why3_vc filter_def by (simp add: Why3_Set.filter_def)
 
-why3_vc choose_spec
-  using assms
-  by (auto simp add: fchoose_def is_empty_def intro: someI_ex)
+why3_vc cardinal_map
+  apply (simp add: fcard_def card_def)
+  by (metis card_def card_image_le finite_fset)
 
-why3_vc is_empty_spec
-  by (simp add: Why3_Set.is_empty_def)
+why3_vc cardinal_diff
+  by (smt fcard_funion_fsubset fcard_mono finter_lower1 fminus_finter2 inf.idem inf_commute int_ops(6) of_nat_mono)
+
+why3_vc mem_singleton
+  using assms by auto
+
+why3_vc subset_filter
+  by (simp add: Fset.subset_def Why3_Set.filter_def)
+
+why3_vc cardinal_union
+  by (smt fcard_funion_finter of_nat_add)
+
+why3_vc empty_is_empty
+  by (meson Fset.is_empty_def assms bot.extremum_uniqueI fsubsetI)
+
+why3_vc is_empty_empty
+  by (simp add: cardinal_empty)
+
+why3_vc subset_inter_1
+  by (simp add: Fset.subset_def)
+
+why3_vc subset_inter_2
+  by (simp add: Fset.subset_def)
+
+why3_vc subset_union_1
+  by (simp add: Fset.subset_def)
+
+why3_vc subset_union_2
+  by (simp add: Fset.subset_def)
+
+why3_vc cardinal_filter
+  using cardinal_subset subset_filter by blast
+
+why3_vc disjoint_diff_eq
+  by (smt Fset.disjoint_def Fset.facts.diff_def fsubsetI fsubset_antisym)
+
+why3_vc  disjoint_diff_s2
+  by (simp add: Fset.facts.disjoint_diff_eq)
+
+why3_vc disjoint_inter_empty
+  by (metis Fset.facts.disjoint_diff_eq Fset.facts.empty_is_empty Fset.facts.is_empty_empty fminus_disjoint fminus_triv) 
+
+why3_vc cardinal_inter_disjoint
+  by (meson Fset.facts.disjoint_inter_empty assms cardinal_empty)
 
 why3_end
 
